proof: dafny

lockserver/proof_definitions.dfy
@@ -34,6 +34,8 @@ predicate Inv(cons:Constants, ds:DistrSys)
 {
     && Trivialities(cons, ds)
     && Safety(cons, ds)
+    && ServerHeld_Implies_Granted(cons, ds)
+    && Granted_Implies_ClientEpochSeen(cons, ds)
     && ClientWorking_Implies_NoMatchingRelease(cons, ds)
     && NoMatchingRelease_Implies_ServerLocked(cons, ds)
     && ServerLocked_Implies_AtMostOneNonMatchedGrant(cons, ds)
@@ -44,7 +46,7 @@ predicate Trivialities(cons:Constants, ds:DistrSys) {
     && cons.WF() 
     && ds.WF(cons)
     && ValidPackets(cons, ds)
-    && Granted_Implies_EpochSeen(cons, ds)
+    
 }
 
 predicate ValidPackets(cons:Constants, ds:DistrSys) 
@@ -61,13 +63,22 @@ predicate ValidPackets(cons:Constants, ds:DistrSys)
 
 /* If a server s has granted to client c, then c in s.epoch_map, 
    and s.epoch_map[c] >= grant_msg.epoch */
-predicate Granted_Implies_EpochSeen(cons:Constants, ds:DistrSys) 
+predicate Granted_Implies_ClientEpochSeen(cons:Constants, ds:DistrSys) 
     requires cons.WF() && ds.WF(cons)
     requires ValidPackets(cons, ds)
 {
     forall p | p in ds.network.sentPackets && p.msg.Grant? :: 
     && p.dst in ds.servers[p.src.idx].epoch_map
     && ds.servers[p.src.idx].epoch_map[p.dst] >= p.msg.e
+}
+
+/* If a server s has resource=Held(c), s has Granted to c */
+predicate ServerHeld_Implies_Granted(cons:Constants, ds:DistrSys) 
+    requires cons.WF() && ds.WF(cons)
+{
+    forall sidx | cons.ValidServerIdx(sidx) && ds.servers[sidx].resource.Held?
+    :: var s := ds.servers[sidx];
+    Packet(s.id, s.resource.client, Grant(s.epoch_map[s.resource.client])) in ds.network.sentPackets
 }
 
 /* For each client c in Working(s) and epoch e, there exists a Grant(s, c, e) with no 
@@ -97,7 +108,7 @@ predicate NoMatchingRelease_Implies_ServerLocked(cons:Constants, ds:DistrSys)
 predicate ServerLocked_Implies_Granted(cons:Constants, ds:DistrSys) 
     requires cons.WF() && ds.WF(cons)
     requires ValidPackets(cons, ds)
-    requires Granted_Implies_EpochSeen(cons, ds)
+    requires Granted_Implies_ClientEpochSeen(cons, ds)
 {
     forall sidx | 
         && cons.ValidServerIdx(sidx) 
@@ -120,7 +131,7 @@ predicate ServerHasAtMostOneNonMatchedGrant(cons:Constants, ds:DistrSys, sidx:in
     requires cons.WF() && ds.WF(cons)
     requires cons.ValidServerIdx(sidx) 
     requires ds.servers[sidx].resource.Held?
-    requires Granted_Implies_EpochSeen(cons, ds)
+    requires Granted_Implies_ClientEpochSeen(cons, ds)
 {
     var s := ds.servers[sidx];
     var possibly_unpaired_grant := GetLatestGrant(s);
